src/ConfigError.v
@@ -1,0 +1,687 @@
+From Coq Require Import
+     Classes.Morphisms
+     Relations.Relation_Operators
+     Logic.JMeq
+     Lists.List
+     Arith.PeanoNat
+     Logic.FunctionalExtensionality.
+
+Require Import ExtLib.Structures.Monads.
+Require Import ExtLib.Data.Monads.OptionMonad.
+
+From Heapster Require Export
+     Permissions
+     Memory.
+
+Import MonadNotation.
+Import ListNotations.
+
+Variant Lifetime := current | finished.
+
+Record config : Type :=
+  {
+  l : list Lifetime;
+  m : memory;
+  }.
+Module Config <: Permissions.Config.
+  Definition t := config.
+End Config.
+
+Definition start_config :=
+  {|
+  l := nil;
+  m := fun _ => None;
+  |}.
+
+Module Permissions' := Permissions Config.
+Export Config.
+Export Permissions'.
+
+(** lifetime helpers **)
+
+Definition lifetime : config -> nat -> option Lifetime :=
+  fun c => nth_error (l c).
+
+Fixpoint replace_list_index {A : Type} (l : list A) (n : nat) (new : A) :=
+  match l with
+  | [] => repeat new (n + 1)
+  | h :: t => match n with
+            | O => new :: t
+            | S n => h :: replace_list_index t n new
+            end
+  end.
+Definition replace_lifetime (c : config) (n : nat) (new : Lifetime) : config :=
+  {|
+  l := replace_list_index (l c) n new;
+  m := m c;
+  |}.
+
+Lemma replace_lifetime_same c n l :
+  lifetime c n = Some l -> replace_lifetime c n l = c.
+Proof.
+  intros. destruct c. unfold lifetime in H. unfold replace_lifetime. f_equal. simpl in *.
+  generalize dependent n. induction l0; intros; simpl in *; auto.
+  - assert (@nth_error Lifetime [] n <> None). intro. rewrite H in H0. discriminate H0.
+    apply nth_error_Some in H0. inversion H0.
+  - destruct n; auto.
+    + inversion H. auto.
+    + rewrite IHl0; auto.
+Qed.
+
+Lemma lifetime_replace_lifetime c n l :
+  lifetime (replace_lifetime c n l) n = Some l.
+Proof.
+  destruct c. unfold replace_lifetime. simpl. revert n l.
+  induction l0; intros; simpl; induction n; auto.
+  unfold lifetime in *. simpl in *. auto.
+Qed.
+
+Definition lifetime_lte (l1 l2 : option Lifetime) : Prop :=
+  match l1, l2 with
+  | None, _ => True
+  | Some current, None => False
+  | Some current, _ => True
+  | Some finished, Some finished => True
+  | _, _ => False
+  end.
+
+Instance lifetime_lte_preorder : PreOrder lifetime_lte.
+Proof.
+  constructor; repeat intro.
+  - destruct x as [[] |]; simpl; auto.
+  - destruct x as [[] |], y as [[] |], z as [[] |]; simpl; intuition.
+Qed.
+
+Definition monotonic_at (p : perm) (n : nat) (x y : config) : Prop :=
+  guar p x y -> lifetime_lte (lifetime x n) (lifetime y n).
+
+Instance monotonic_at_reflexive p n : Reflexive (monotonic_at p n).
+Proof.
+  repeat intro. reflexivity.
+Qed.
+
+Lemma bottom_monotonic_at n : forall x y, monotonic_at bottom_perm n x y.
+Proof.
+  repeat intro. simpl in H. subst. reflexivity.
+Qed.
+
+Definition monotonic (P : Perms) (n : nat) : Prop :=
+  forall p, p ∈ P -> exists p', p' <= p /\ p' ∈ P /\ forall x y, monotonic_at p' n x y.
+
+Lemma monotonic_bottom n : monotonic bottom_Perms n.
+Proof.
+  repeat intro. exists bottom_perm. split; [| split].
+  apply bottom_perm_is_bottom. auto. apply bottom_monotonic_at.
+Qed.
+
+Program Definition restrict_monotonic_at (p : perm) (n : nat) : perm :=
+  {|
+  pre := pre p;
+  rely := rely p;
+  guar := fun x y => guar p x y /\ monotonic_at p n x y;
+  |}.
+Next Obligation.
+  respects.
+Qed.
+Next Obligation.
+  constructor; repeat intro.
+  - split; intuition.
+  - destruct H, H0. split; [etransitivity; eauto |]. intro. etransitivity; eauto.
+Qed.
+
+Lemma restrict_monotonic_at_monotone p p' n :
+  p <= p' -> restrict_monotonic_at p n <= restrict_monotonic_at p' n.
+Proof.
+  intros []. constructor; intros; simpl; auto. destruct H.
+  split; auto. intro. auto.
+Qed.
+
+Lemma restrict_monotonic_at_lte p n : restrict_monotonic_at p n <= p.
+Proof.
+  constructor; intros; simpl in *; intuition.
+Qed.
+
+Definition invariant_at (p : perm) (n : nat) : Prop :=
+  forall l1 l2 x y, guar p x y <-> guar p (replace_lifetime x n l1) (replace_lifetime y n l2).
+
+Lemma invariant_l p n (Hinv : invariant_at p n) :
+  forall l1 l2 x y, lifetime y n = Some l2 ->
+               guar p x y <-> guar p (replace_lifetime x n l1) y.
+Proof.
+  intros.
+  rewrite <- (replace_lifetime_same y n l2) at 2; auto.
+Qed.
+
+Lemma invariant_r p n (Hinv : invariant_at p n) :
+  forall l1 l2 x y, lifetime x n = Some l1 ->
+               guar p x y <-> guar p x (replace_lifetime y n l2).
+Proof.
+  intros.
+  rewrite <- (replace_lifetime_same x n l1) at 2; auto.
+Qed.
+
+(** memory helpers **)
+
+(* read c at memory location ptr. ptr must be a valid location and allocated. *)
+Definition read (c : config) (ptr : addr)
+  : option SByte :=
+  match m c (fst ptr) with
+  | Some (LBlock size bytes) => if snd ptr <? size then bytes (snd ptr) else None
+  | _ => None
+  end.
+
+(* TODO clean up *)
+Definition config_mem (ptr : addr) (v : SByte) :=
+  {|
+  l := nil;
+  m := fun b => if b =? (fst ptr)
+             then Some (LBlock (snd ptr + 1) (fun o => if o =? (snd ptr)
+                                                    then Some v
+                                                    else None))
+             else None;
+  |}.
+Lemma read_config_mem l v : read (config_mem l v) l = Some v.
+Proof.
+  destruct l as [b o]. unfold read, config_mem. simpl. repeat rewrite Nat.eqb_refl.
+  assert (o < o + 1). rewrite Nat.add_1_r. apply Nat.lt_succ_diag_r.
+  pose proof Nat.ltb_spec0.
+  eapply Bool.reflect_iff in H0. rewrite H0 in H. rewrite H. reflexivity.
+Qed.
+
+Definition is_some {A} (o : option A) : bool :=
+  match o with
+  | Some _ => true
+  | None => false
+  end.
+
+Definition allocated (c : config) (ptr : addr) : Prop :=
+  match m c (fst ptr) with
+  | Some (LBlock size bytes) =>
+    match bytes (snd ptr) with
+    | Some _ => snd ptr < size
+    | _ => False
+    end
+  | _ => False
+  end.
+
+Definition alloc_invariant (c1 c2 : config) (ptr : addr) : Prop :=
+  allocated c1 ptr = allocated c2 ptr.
+
+Lemma alloc_invariant_read c1 c2 ptr :
+  alloc_invariant c1 c2 ptr ->
+  read c2 ptr = None ->
+  read c1 ptr = None.
+Proof.
+  destruct ptr as [b o].
+  unfold alloc_invariant. unfold allocated. unfold read. simpl in *. intros.
+  destruct (m c1 b), (m c2 b); try solve [inversion H0]; auto.
+  - destruct l0, l1.
+    destruct (bytes o), (bytes0 o).
+    + destruct (o <? size) eqn:?; auto.
+      rewrite <- (Bool.reflect_iff _ _ (Nat.ltb_spec0 _ _)) in Heqb0.
+      rewrite H in Heqb0.
+      rewrite (Bool.reflect_iff _ _ (Nat.ltb_spec0 _ _)) in Heqb0.
+      rewrite Heqb0 in H0. inversion H0.
+    + destruct (o <? size) eqn:?; auto.
+      rewrite <- (Bool.reflect_iff _ _ (Nat.ltb_spec0 _ _)) in Heqb0.
+      rewrite H in Heqb0. inversion Heqb0.
+    + destruct (o <? size); auto.
+    + destruct (o <? size); auto.
+  - destruct l0. destruct (bytes o).
+    + destruct (o <? size) eqn:?; auto.
+      rewrite <- (Bool.reflect_iff _ _ (Nat.ltb_spec0 _ _)) in Heqb0.
+      rewrite H in Heqb0. inversion Heqb0.
+    + destruct (o <? size); auto.
+Qed.
+
+(* write val to c at memory location ptr. ptr must be a valid location and allocated. *)
+Definition write (c : config) (ptr : addr) (val : SByte)
+  : option config :=
+  match m c (fst ptr) with
+  | Some (LBlock size bytes) =>
+    if andb (snd ptr <? size) (is_some (bytes (snd ptr)))
+    then Some {|
+             l := l c;
+             m := fun b => if b =? fst ptr
+                        then Some (LBlock size (fun o => if o =? snd ptr
+                                                      then Some val
+                                                      else bytes o))
+                        else m c b;
+           |}
+    else None
+  | _ => None
+  end.
+
+Lemma write_config_mem l v v' : write (config_mem l v) l v' = Some (config_mem l v').
+Proof.
+  destruct l as [b o]. unfold write, config_mem. simpl. repeat rewrite Nat.eqb_refl.
+  assert (o < o + 1). rewrite Nat.add_1_r. apply Nat.lt_succ_diag_r.
+  pose proof Nat.ltb_spec0.
+  eapply Bool.reflect_iff in H0. rewrite H0 in H. rewrite H. simpl.
+  do 2 f_equal. apply functional_extensionality. intros.
+  destruct (x =? b); auto. do 2 f_equal. apply functional_extensionality. intros.
+  destruct (x0 =? o); auto.
+Qed.
+
+Lemma write_success_allocation c c' ptr val :
+  write c ptr val = Some c' ->
+  alloc_invariant c c' ptr.
+Proof.
+  destruct ptr as [b o].
+  intros. unfold alloc_invariant. unfold allocated. unfold write in H. simpl in *.
+  destruct (m c b) eqn:?; try solve [inversion H]. destruct l0.
+  destruct (o <? size) eqn:?; try solve [inversion H].
+  destruct (is_some (bytes o)) eqn:?; try solve [inversion H].
+  inversion H; subst; clear H. simpl. repeat rewrite Nat.eqb_refl.
+  destruct (bytes o); auto. inversion Heqb1.
+Qed.
+
+Lemma write_success_ptr c c' ptr val :
+  write c ptr val = Some c' ->
+  read c' ptr = Some val.
+Proof.
+  intros. destruct ptr as [b o]. unfold read, write in *. simpl in *.
+  destruct (m c b); try solve [inversion H]. destruct l0.
+  destruct (o <? size) eqn:?, (is_some (bytes o)) eqn:?; simpl in *; inversion H; simpl in *.
+  repeat rewrite Nat.eqb_refl. rewrite Heqb0. auto.
+Qed.
+
+Lemma write_success_other_ptr c c' ptr val :
+  write c ptr val = Some c' ->
+  forall ptr', ptr <> ptr' -> read c ptr' = read c' ptr'.
+Proof.
+  destruct ptr as [b o].
+  unfold write. unfold read. simpl. intros.
+  destruct (m c b) eqn:?; try solve [inversion H]. destruct l0.
+  destruct (o <? size) eqn:?; try solve [inversion H].
+  destruct (is_some (bytes o)) eqn:?; try solve [inversion H].
+  inversion H; subst; clear H. destruct ptr' as [b' o']. simpl.
+  destruct (addr_neq_cases b b' o o' H0).
+  - rewrite (Bool.reflect_iff _ _ (Nat.eqb_spec _ _)) in H.
+    apply Bool.not_true_is_false in H. rewrite Nat.eqb_sym.
+    rewrite H. reflexivity.
+  - destruct (b' =? b) eqn:?; auto.
+    rewrite <- (Bool.reflect_iff _ _ (Nat.eqb_spec _ _)) in Heqb2. subst.
+    rewrite Heqo0.
+    rewrite (Bool.reflect_iff _ _ (Nat.eqb_spec _ _)) in H.
+    apply Bool.not_true_is_false in H. rewrite Nat.eqb_sym.
+    rewrite H. reflexivity.
+Qed.
+
+Lemma write_success_others c c' ptr val :
+  write c ptr val = Some c' ->
+  l c = l c'.
+Proof.
+  destruct ptr as [b o].
+  unfold write. simpl. intros.
+  destruct (m c b); try solve [inversion H].
+  destruct l0. destruct ((o <? size) && is_some (bytes o))%bool; try solve [inversion H].
+  inversion H; subst; simpl. split; auto.
+Qed.
+
+Lemma write_read : forall c c' ptr val,
+    write c ptr val = Some c' ->
+    read c' ptr = Some val.
+Proof.
+  intros. destruct ptr as [b o].
+  unfold write, read in *. simpl in *.
+  destruct (m c b); try solve [inversion H]. destruct l0.
+  destruct (o <? size) eqn:?; try solve [inversion H].
+  destruct (bytes o); try solve [inversion H]. simpl in *. inversion H; simpl.
+  repeat rewrite Nat.eqb_refl. rewrite Heqb0. reflexivity.
+Qed.
+
+(* Lemma read_write : forall c ptr, *)
+(*     (exists val, read c ptr = Some val) -> *)
+(*     bind (read c ptr) (fun val => write c ptr val) = Some c. *)
+(* Proof. *)
+(*   intros. destruct H. simpl. rewrite H. unfold read in H. unfold write. *)
+(*   destruct ptr as (b & o). destruct c. simpl in *. *)
+(*   destruct (m0 b) eqn:?; try solve [inversion H]. destruct l1. *)
+(*   destruct (o <? size); try solve [inversion H]. *)
+(*   apply f_equal. (* not sure why I need apply *) *)
+(*   f_equal. apply functional_extensionality. intros. destruct (x0 =? b) eqn:?; auto. *)
+(*   rewrite <- (Bool.reflect_iff _ _ (Nat.eqb_spec _ _)) in Heqb0; subst. *)
+(*   rewrite Heqo0. f_equal. f_equal. apply functional_extensionality. intros. *)
+(*   destruct (x0 =? o) eqn:?; auto. *)
+(*   rewrite <- (Bool.reflect_iff _ _ (Nat.eqb_spec _ _)) in Heqb0. subst. auto. *)
+(* Qed. *)
+
+(* Lemma write_write : forall c ptr val, *)
+(*     bind (write c ptr val) (fun c' => write c' ptr val) = write c ptr val. *)
+(* Proof. *)
+(*   simpl. intros. destruct (write c ptr val) eqn:?; auto. unfold write in *. *)
+(*   destruct (m c (fst ptr)) eqn:?; try solve [inversion Heqo]. *)
+(*   destruct l0 eqn:?. destruct (snd ptr <? size) eqn:?; inversion Heqo. *)
+(*   simpl. rewrite Nat.eqb_refl. rewrite Heqb. apply f_equal. f_equal. *)
+(*   apply functional_extensionality. intros. destruct (x =? fst ptr); auto. *)
+(*   repeat f_equal. apply functional_extensionality. intros. *)
+(*   destruct (x0 =? snd ptr); auto. *)
+(* Qed. *)
+
+(** Lifetime permissions **)
+
+Program Definition when (n : nat) (p : perm) : perm :=
+  {|
+  pre := fun x => (lifetime x n = Some current /\ pre p x) \/
+               lifetime x n = Some finished;
+  rely := fun x y => lifetime x n = None /\ lifetime y n = None \/
+                  lifetime y n = Some finished \/
+                  lifetime x n = Some current /\ lifetime y n = Some current /\ rely p x y;
+  guar := fun x y => x = y \/
+                 lifetime x n = Some current /\ lifetime y n = Some current /\ guar p x y;
+  |}.
+Next Obligation.
+  constructor; repeat intro.
+  - destruct (lifetime x n) as [[] |]; intuition.
+  - decompose [and or] H; decompose [and or] H0; subst; auto.
+    + rewrite H1 in H3. discriminate H3.
+    + rewrite H2 in H3. discriminate H3.
+    + rewrite H1 in H2. discriminate H2.
+    + rewrite H2 in H5. discriminate H5.
+    + right; right. split; [| split]; auto. etransitivity; eauto.
+Qed.
+Next Obligation.
+  decompose [and or] H; decompose [or and] H0; subst; auto.
+  - rewrite H2 in H4. discriminate H4.
+  - rewrite H1 in H2. discriminate H2.
+  - left. split; auto. eapply pre_respects; eauto.
+  - rewrite H1 in H3. discriminate H3.
+Qed.
+Next Obligation.
+  constructor; repeat intro; auto.
+  decompose [and or] H; decompose [and or] H0; subst; auto.
+  right. split; [| split]; auto. etransitivity; eauto.
+Qed.
+
+Lemma when_monotone n p1 p2 : p1 <= p2 -> when n p1 <= when n p2.
+Proof.
+  intros. destruct H. constructor; simpl; intros; decompose [and or] H; auto 7.
+Qed.
+
+Instance Proper_lte_perm_when :
+  Proper (eq ==> lte_perm ==> lte_perm) when.
+Proof.
+  repeat intro; subst. apply when_monotone; auto.
+Qed.
+
+Instance Proper_eq_perm_when :
+  Proper (eq ==> eq_perm ==> eq_perm) when.
+Proof.
+  repeat intro; subst. split; apply when_monotone; auto.
+Qed.
+
+Lemma restrict_monotonic_at_when p n : when n p ≡ restrict_monotonic_at (when n p) n.
+Proof.
+  split; [constructor; intros; simpl in *; auto | apply restrict_monotonic_at_lte].
+  decompose [and or] H; subst; try solve [intuition]. split; auto.
+  intro. rewrite H1, H0. reflexivity.
+Qed.
+Lemma when_restrict_monotonic_at p n : when n p ≡ when n (restrict_monotonic_at p n).
+Proof.
+  split; constructor; intros; simpl in *; intuition.
+  right; intuition. intro. rewrite H, H0. reflexivity.
+Qed.
+
+Program Definition owned (n : nat) (p : perm) : perm :=
+  {|
+  pre := fun x => lifetime x n = Some current;
+  rely := fun x y => lifetime x n = lifetime y n /\ (lifetime x n = Some finished -> rely p x y);
+  guar := fun x y => x = y \/
+                 lifetime y n = Some finished /\ guar p (replace_lifetime x n finished) y;
+  |}.
+Next Obligation.
+  constructor; repeat intro; auto.
+  - split; intuition.
+  - destruct H, H0.
+    split; etransitivity; eauto. apply H2. rewrite <- H. auto.
+Qed.
+Next Obligation.
+  constructor; repeat intro; auto.
+  decompose [and or] H; decompose [and or] H0; subst; auto.
+  right. split; auto. etransitivity; eauto.
+  rewrite <- (replace_lifetime_same y n finished); auto.
+Qed.
+
+Lemma owned_monotone n p1 p2 : p1 <= p2 -> owned n p1 <= owned n p2.
+Proof.
+  intros. destruct H. constructor; simpl; intros; decompose [and or] H; auto 6.
+Qed.
+
+Instance Proper_lte_perm_owned :
+  Proper (eq ==> lte_perm ==> lte_perm) owned.
+Proof.
+  repeat intro; subst. apply owned_monotone; auto.
+Qed.
+
+Instance Proper_eq_perm_owned :
+  Proper (eq ==> eq_perm ==> eq_perm) owned.
+Proof.
+  repeat intro; subst. split; apply owned_monotone; auto.
+Qed.
+
+Lemma restrict_monotonic_at_owned p n : owned n p ≡ restrict_monotonic_at (owned n p) n.
+Proof.
+  split; [constructor; intros; simpl in *; auto | apply restrict_monotonic_at_lte].
+  decompose [and or] H; subst; try solve [intuition]. split; auto. clear H.
+  intro. rewrite H1. destruct (lifetime x n) as [[] |]; simpl; auto.
+Qed.
+Lemma owned_restrict_monotonic_at p n : owned n p ≡ owned n (restrict_monotonic_at p n).
+Proof.
+  split; constructor; intros; simpl in *; intuition.
+  right; intuition. intro. rewrite H. rewrite lifetime_replace_lifetime. reflexivity.
+Qed.
+
+(* trivial direction *)
+Lemma foo' p q n :
+  owned n (restrict_monotonic_at p n * restrict_monotonic_at q n) <=
+  owned n (restrict_monotonic_at (p * q) n).
+Proof.
+  rewrite <- owned_restrict_monotonic_at. apply owned_monotone.
+  apply sep_conj_perm_monotone; apply restrict_monotonic_at_lte.
+Qed.
+
+Lemma lifetimes_sep_gen p q n :
+  p ⊥ owned n q -> when n p ⊥ owned n (p * q).
+Proof.
+  split; intros.
+  - simpl in H0. decompose [and or] H0. subst; intuition.
+    simpl. right; left; auto.
+  - simpl in H0. decompose [and or] H0. subst; intuition.
+    simpl. split. rewrite H1, H2; auto.
+    intros. rewrite H2 in H3. discriminate H3.
+Qed.
+
+(* not actually a special case of the above *)
+Lemma lifetimes_sep n p : when n p ⊥ owned n p.
+Proof.
+  constructor; intros; simpl in H; auto.
+  - decompose [and or] H; subst; try reflexivity.
+    simpl. right; left; auto.
+  - decompose [and or] H; subst; try reflexivity.
+    simpl. split. rewrite H1, H0. auto. intros. rewrite H1 in H2. discriminate H2.
+Qed.
+
+Lemma convert p q n (Hmon : forall x y, monotonic_at p n x y) (Hmon' : forall x y, monotonic_at q n x y) :
+  when n p * owned n (p * q) <= p * owned n q.
+Proof.
+  split; intros.
+  - simpl in *. decompose [and or] H; auto. split; auto. split; auto.
+    eapply lifetimes_sep_gen; eauto.
+  - simpl in *. decompose [and or] H; auto. destruct (lifetime x n) as [[] | ]; auto 7.
+  - simpl in H. induction H. 2: { econstructor 2; eauto. }
+    decompose [and or] H; simpl; subst; try solve [constructor; auto].
+    clear H.
+    apply Operators_Properties.clos_trans_t1n_iff.
+    apply Operators_Properties.clos_trans_t1n_iff in H2.
+    constructor 2 with (y:=replace_lifetime x n finished).
+    { right; right. split; [apply lifetime_replace_lifetime | reflexivity]. }
+    pose proof (lifetime_replace_lifetime x n finished).
+    induction H2; intros; subst; auto.
+    + constructor. destruct H1; auto. right; right. split; auto.
+      rewrite replace_lifetime_same; auto.
+    + assert (lifetime y n = Some finished).
+      { destruct H1; [apply Hmon in H1 | apply Hmon' in H1]; rewrite H in H1; simpl in H1;
+          destruct (lifetime y n) as [[] |]; inversion H1; auto. }
+      econstructor 2. 2: apply IHclos_trans_1n; auto.
+      destruct H1; auto. right; right. split; auto. rewrite replace_lifetime_same; auto.
+Qed.
+
+(* special case of convert *)
+Lemma convert_bottom p n (Hmon : forall x y, monotonic_at p n x y) :
+  when n p * owned n p <= p * owned n bottom_perm.
+Proof.
+  rewrite <- (sep_conj_perm_bottom p) at 2. apply convert; auto.
+  repeat intro. simpl in H. subst. reflexivity.
+Qed.
+
+(** memory permissions **)
+
+(* Program Definition read_p (ptr : addr) : perm := *)
+(*   {| *)
+(*   (* ptr points to valid memory *) *)
+(*   pre x := exists v, read x ptr = Some v; *)
+(*   (* only checks if the memory ptr points to in the 2 configs are equal *) *)
+(*   rely x y := alloc_invariant x y ptr; *)
+(*   (* read x ptr = None <-> read y ptr = None; *) *)
+(*   (* only the pointer we have write permission to may change *) *)
+(*   guar x y := x = y; *)
+(*   |}. *)
+(* Next Obligation. *)
+(*   constructor; unfold alloc_invariant; unfold allocated; repeat intro; auto. *)
+(*   destruct (m x (fst ptr)), (m y (fst ptr)), (m z (fst ptr)); intuition. *)
+(*   - destruct l0, l1, l2. *)
+(*     destruct (bytes (snd ptr)), (bytes0 (snd ptr)), (bytes1 (snd ptr)); subst; *)
+(*       etransitivity; eauto. *)
+(*   - destruct l0, l1. *)
+(*     destruct (bytes (snd ptr)), (bytes0 (snd ptr)); subst; *)
+(*       etransitivity; eauto. *)
+(*   - destruct l0, l1. *)
+(*     destruct (bytes (snd ptr)), (bytes0 (snd ptr)); subst; *)
+(*       etransitivity; eauto. *)
+(*   - destruct l0, l1. *)
+(*     destruct (bytes (snd ptr)), (bytes0 (snd ptr)); subst; *)
+(*       etransitivity; eauto. *)
+(* Qed. *)
+(* Next Obligation. *)
+(*   destruct (read y ptr) eqn:?. *)
+(*   eexists; eauto. *)
+(*   assert ((None : option SByte) = None) by reflexivity. *)
+(*   eapply alloc_invariant_read in Heqo; eauto. rewrite H1 in Heqo. inversion Heqo. *)
+(* Qed. *)
+(* Next Obligation. *)
+(*   constructor; repeat intro; auto. etransitivity; eauto. *)
+(* Qed. *)
+
+(* (* TODO factor out common pre and rely *) *)
+(* Program Definition write_p (ptr : addr) : perm := *)
+(*   {| *)
+(*   (* ptr points to valid memory *) *)
+(*   pre x := exists v, read x ptr = Some v; *)
+(*   (* only checks if the memory ptr points to in the 2 configs are equal *) *)
+(*   rely x y := read x ptr = read y ptr; *)
+(*   (* only the pointer we have write permission to may change *) *)
+(*   (* TODO: cannot dealloc or alloc here... *) *)
+(*   guar x y := (forall ptr', ptr <> ptr' -> read x ptr' = read y ptr') /\ *)
+(*              alloc_invariant x y ptr; *)
+(*   |}. *)
+(* Next Obligation. *)
+(*   constructor; repeat intro; auto. etransitivity; eauto. *)
+(* Qed. *)
+(* Next Obligation. *)
+(*   eexists; eauto. *)
+(* Qed. *)
+(* Next Obligation. *)
+(*   constructor; split; repeat intro; try solve [intuition]. *)
+(*   - reflexivity. *)
+(*   - destruct H, H0. etransitivity. apply H; auto. auto. *)
+(*   - destruct H, H0. etransitivity. apply H1. auto. *)
+(* Qed. *)
+
+Program Definition read_perm (ptr : addr) (v : SByte) : perm :=
+  {|
+  (* ptr points to valid memory *)
+  pre x := read x ptr = Some v;
+  (* only checks if the memory ptr points to in the 2 configs are equal *)
+  rely x y := read x ptr = read y ptr;
+  (* no guarates allowed *)
+  guar x y := x = y;
+  |}.
+Next Obligation.
+  constructor; repeat intro; auto. etransitivity; eauto.
+Qed.
+Next Obligation.
+  constructor; repeat intro; subst; auto.
+Qed.
+
+Program Definition write_perm (ptr : addr) (v : SByte) : perm :=
+  {|
+  (* ptr points to valid memory *)
+  pre x := read x ptr = Some v;
+  (* only checks if the memory ptr points to in the 2 configs are equal *)
+  rely x y := read x ptr = read y ptr;
+  (* only the pointer we have write permission to may change *)
+  guar x y := (forall ptr', ptr <> ptr' -> read x ptr' = read y ptr') /\
+             alloc_invariant x y ptr /\
+             l x = l y;
+  |}.
+Next Obligation.
+  constructor; repeat intro; auto. etransitivity; eauto.
+Qed.
+Next Obligation.
+  constructor; split; repeat intro; try solve [intuition].
+  - split; [| split]; reflexivity.
+  - destruct H, H0. etransitivity. apply H; auto. auto.
+  - destruct H as (? & ? & ?), H0 as (? & ? & ?).
+    split; etransitivity; eauto.
+Qed.
+
+Definition read_Perms (ptr : addr) (P : SByte -> Perms) : Perms :=
+  meet_Perms (fun Q => exists y : SByte, Q = singleton_Perms (read_perm ptr y) ** P y).
+
+Definition write_Perms (ptr : addr) (P : SByte -> Perms) : Perms :=
+  meet_Perms (fun Q => exists y : SByte, Q = singleton_Perms (write_perm ptr y) ** P y).
+
+Lemma read_lte_write : forall ptr v, read_perm ptr v <= write_perm ptr v.
+Proof.
+  constructor; simpl; repeat intro; subst; auto.
+  split; [| split; [| split]]; intros; reflexivity.
+Qed.
+
+Lemma read_write_separate_neq_ptr : forall ptr ptr' v v',
+    read_perm ptr v ⊥ write_perm ptr' v' <-> ptr <> ptr'.
+Proof.
+  split; repeat intro.
+  - destruct H as [? _]. simpl in *. subst.
+    specialize (sep_l0 (config_mem ptr' (Byte 0)) (config_mem ptr' (Byte 1))).
+    do 2 rewrite read_config_mem in sep_l0.
+    assert (Some (Byte 0) = Some (Byte 1) -> False) by inversion 1.
+    apply H. clear H. apply sep_l0. split; [| split; [| split]]; auto.
+    + intros. unfold read, config_mem. simpl.
+      destruct ptr', ptr'0. destruct (addr_neq_cases _ _ _ _ H); simpl in *.
+      * rewrite (Bool.reflect_iff _ _ (Nat.eqb_spec _ _)) in H0.
+        apply Bool.not_true_is_false in H0. rewrite Nat.eqb_sym in H0.
+        rewrite H0. auto.
+      * destruct (n1 =? n); auto. destruct (n2 <? n0 + 1); auto.
+        rewrite (Bool.reflect_iff _ _ (Nat.eqb_spec _ _)) in H0.
+        apply Bool.not_true_is_false in H0. rewrite Nat.eqb_sym in H0.
+        rewrite H0. auto.
+    + unfold alloc_invariant, allocated, config_mem. simpl.
+      repeat rewrite Nat.eqb_refl. auto.
+  - constructor; intros; simpl in *; subst; auto.
+    destruct H0. auto.
+Qed.
+
+Lemma write_write_separate_neq_ptr : forall ptr ptr' v v',
+    write_perm ptr v ⊥ write_perm ptr' v' <-> ptr <> ptr'.
+Proof.
+  split; intros.
+  - symmetry in H. eapply separate_antimonotone in H. symmetry in H.
+    eapply read_write_separate_neq_ptr. apply H. apply read_lte_write.
+  - constructor; intros; simpl in *; destruct H0; auto.
+Qed.
+
+Lemma read_separate : forall ptr ptr' v v', read_perm ptr v ⊥ read_perm ptr' v'.
+Proof.
+  constructor; intros; simpl in *; subst; reflexivity.
+Qed.
