src/Functional.v
@@ -1,0 +1,114 @@
+From Heapster Require Import
+     Permissions
+     Config.
+     (* StepError. *)
+     (* Typing. *)
+
+From ITree Require Import
+     ITree
+     ITreeFacts
+     Basics.MonadState
+     Basics.MonadProp
+     Events.State
+     Events.Exception
+     Events.Nondeterminism
+     Eq.Eq
+     Eq.UpToTaus
+     Eq.EqAxiom.
+
+From Paco Require Import
+     paco.
+
+Section bisim.
+  Variant ModifyE {C : Type} : Type -> Type :=
+  | Modify : forall (f : C -> C), ModifyE C
+  .
+
+  Definition E (C : Type) := (exceptE unit +' @ModifyE C +' nondetE).
+
+  Context {config specConfig : Type}.
+
+  (* todo move somewhere else *)
+  Definition sep_step (p q : @perm config specConfig) : Prop :=
+    forall r, p ⊥ r -> q ⊥ r.
+
+  Inductive typing_gen {R1 R2 : Type} typing (p : perm) (Q : R1 -> R2 -> Perms) :
+    itree (E config) R1 -> config -> itree (E specConfig) R2 -> specConfig -> Prop :=
+  | typing_ret r1 c1 r2 c2 :
+      pre p c1 c2 ->
+      p ∈ Q r1 r2 ->
+      typing_gen typing p Q (Ret r1) c1 (Ret r2) c2
+  | typing_err t1 c1 c2 :
+      typing_gen typing p Q t1 c1 (throw tt) c2
+  | typing_tau_L t1 c1 t2 c2 :
+      pre p c1 c2 ->
+      typing_gen typing p Q t1 c1 t2 c2 ->
+      typing_gen typing p Q (Tau t1) c1 t2 c2
+  | typing_tau_R t1 c1 t2 c2 :
+      pre p c1 c2 ->
+      typing_gen typing p Q t1 c1 t2 c2 ->
+      typing_gen typing p Q t1 c1 (Tau t2) c2
+  | typing_tau t1 c1 t2 c2 :
+      pre p c1 c2 ->
+      typing p Q t1 c1 t2 c2 ->
+      typing_gen typing p Q (Tau t1) c1 (Tau t2) c2
+  | typing_modify_L f k c1 t2 c2 p' :
+      pre p c1 c2 ->
+      guar p c1 (f c1) ->
+      sep_step p p' ->
+      typing_gen typing p' Q (k c1) (f c1) t2 c2 ->
+      typing_gen typing p Q (vis (Modify f) k) c1 t2 c2
+  | typing_modify_R t1 c1 f k c2 p' :
+      pre p c1 c2 ->
+      sep_step p p' ->
+      typing_gen typing p Q t1 c1 (k c2) (f c2) ->
+      typing_gen typing p Q t1 c1 (vis (Modify f) k) c2
+  | typing_modify f1 k1 c1 f2 k2 c2 p' :
+      pre p c1 c2 ->
+      guar p c1 (f1 c1) ->
+      sep_step p p' ->
+      typing p Q (k1 c1) (f1 c1) (k2 c2) (f2 c2) ->
+      typing_gen typing p Q (vis (Modify f1) k1) c1 (vis (Modify f2) k2) c2
+  | typing_choice_L k c1 t2 c2 p' :
+      pre p c1 c2 ->
+      sep_step p p' ->
+      (forall b, typing_gen typing p Q (k b) c1 t2 c2) ->
+      typing_gen typing p Q (vis Or k) c1 t2 c2
+  | typing_choice_R t1 c1 k c2 p' :
+      pre p c1 c2 ->
+      sep_step p p' ->
+      (forall b, typing_gen typing p Q t1 c1 (k b) c2) ->
+      typing_gen typing p Q t1 c1 (vis Or k) c2
+  | typing_choice k1 c1 k2 c2 p' :
+      pre p c1 c2 ->
+      sep_step p p' ->
+      (forall b1 b2, typing p Q (k1 b1) c1 (k2 b2) c2) ->
+      typing_gen typing p Q (vis Or k1) c1 (vis Or k2) c2
+  .
+
+  Definition typing {R1 R2} := paco6 (@typing_gen R1 R2) bot6.
+
+End bisim.
+
+
+
+Variant typing_gen {R1 R2 : Type} typing (P : Perms) (Q : R1 -> R2 -> Perms) :
+  itree E R1 -> itree specE R2 -> Prop :=
+| cond : forall t spec, (exists c t' c', step t c t' c') /\ (* we can step *)
+                   (forall p c, p ∈ P ->
+                           pre p c ->
+                           forall t' c',
+                             step t c t' c' -> (* and everything we can step to... *)
+                             (
+                               (* we step to configs that satisfy the perm *)
+                               guar p c c' /\
+                               (* we step to machines that are well-typed by some
+                                  other perm that maintains separation *)
+                               exists spec', spec ≈ spec' /\
+                               exists P', typing P' Q t' spec' /\ exists p', p' ∈ P' /\ p = p' /\ pre p' c')) ->
+                   typing_gen typing P Q t spec
+| err : forall t, typing_gen typing P Q t (throw tt)
+| ret : forall r1 r2, Q r1 r2 ⊑ P -> typing_gen typing P Q (Ret r1) (Ret r2).
+
+(* Definition typing_perm := paco3 typing_perm_gen bot3. *)
+Definition typing {R1 R2} := paco4 (@typing_gen R1 R2) bot4.
